Lots done in Term.thy + skeleton

Term.thy
@@ -73,7 +73,7 @@ next
 next
   case (Sym_encrypt msg1 msg2)
   have "length [embed msg1, embed msg2] = arity SSym_encrypt" by simp
-  then show ?case sledgehammer
+  then show ?case
     by (metis Sym_encrypt.IH(1) Sym_encrypt.IH(2) embed.simps(5) list.discI list.set_cases set_ConsD wf_term.simps)
 next
   case (Public_key_encrypt msg1 msg2)
@@ -156,18 +156,297 @@ lemma msg_of_term_inject:
 (* 5. (d) *)
 
 fun m_fv :: "msg \<Rightarrow> string set" where
+  "m_fv (Cons s) = {}"
+| "m_fv (Var s) = {s}"
+| "m_fv (Hash m) = m_fv m"
+| "m_fv (Pair m1 m2) = m_fv m1 \<union> m_fv m2"
+| "m_fv (Sym_encrypt m1 m2) = m_fv m1 \<union> m_fv m2"
+| "m_fv (Public_key_encrypt m1 m2) = m_fv m1 \<union> m_fv m2"
+| "m_fv (Signature m1 m2) = m_fv m1 \<union> m_fv m2"
 
+lemma link_fv:
+  "m_fv msg = fv (embed msg)"
+  apply (induction msg)
+        apply simp_all
+  done
 
-datatype msg =
-  "m_fv (
+type_synonym m_subst = "char list \<Rightarrow> msg"
+type_synonym m_eq = "msg \<times> msg"
+type_synonym m_eqs = "m_eq list"
+
+fun embed_eq :: "m_eq \<Rightarrow> (symbol, string) equation " where
+  "embed_eq (m1, m2) = (embed m1, embed m2)"
+
+fun m_eq_of_eq :: "(symbol, string) equation \<Rightarrow> m_eq" where
+  "m_eq_of_eq (a, b) = (msg_of_term a, msg_of_term b)"
+
+fun embed_eqs :: "m_eqs \<Rightarrow> (symbol, string) equations" where
+  "embed_eqs [] = []"
+| "embed_eqs (eq # U) = (embed_eq eq) # (embed_eqs U)"
+
+fun m_eqs_of_eqs :: "(symbol, string) equations \<Rightarrow> m_eqs" where
+  "m_eqs_of_eqs [] = []"
+| "m_eqs_of_eqs (eq # U) = (m_eq_of_eq eq) # (m_eqs_of_eqs U)"
+
+fun m_sapply :: "m_subst \<Rightarrow> msg \<Rightarrow> msg"
+  where
+  "m_sapply \<sigma> (Cons s) = Cons s"
+| "m_sapply \<sigma> (Var s) =  \<sigma> s"
+| "m_sapply \<sigma> (Hash m) = Hash (m_sapply \<sigma> m)"
+| "m_sapply \<sigma> (Pair m1 m2) = Pair (m_sapply \<sigma> m1) (m_sapply \<sigma> m2)"
+| "m_sapply \<sigma> (Sym_encrypt m1 m2) = Sym_encrypt (m_sapply \<sigma> m1) (m_sapply \<sigma> m2)"
+| "m_sapply \<sigma> (Public_key_encrypt m1 m2) = Public_key_encrypt (m_sapply \<sigma> m1) (m_sapply \<sigma> m2)"
+| "m_sapply \<sigma> (Signature m1 m2) = Signature (m_sapply \<sigma> m1) (m_sapply \<sigma> m2)"
+
+lemma link_sapply:
+  "m_sapply \<sigma> m = msg_of_term (sapply (embed \<circ> \<sigma>) (embed m))"
+  apply (induction m)
+        apply simp_all
+  done
+
+fun m_sapply_eq :: "m_subst \<Rightarrow> m_eq \<Rightarrow> m_eq" where
+  "m_sapply_eq \<sigma> eq = (m_sapply \<sigma> (fst eq), m_sapply \<sigma> (snd eq))"
+
+lemma link_sapply_eq:
+  "m_sapply_eq \<sigma> eq = m_eq_of_eq (sapply_eq (embed \<circ> \<sigma>) (embed_eq eq))"
+  by (metis embed_eq.simps fstI link_sapply m_eq_of_eq.simps m_sapply_eq.elims prod.collapse sapply_eq.elims sndI)
+
+fun m_sapply_eqs :: "m_subst \<Rightarrow> m_eqs \<Rightarrow> m_eqs" where
+  "m_sapply_eqs \<sigma> [] = []"
+| "m_sapply_eqs \<sigma> (eq # U) = (m_sapply_eq \<sigma> eq) # (m_sapply_eqs \<sigma> U)"
+
+lemma link_sapply_eqs:
+  "m_sapply_eqs \<sigma> U = m_eqs_of_eqs (sapply_eq_system (embed \<circ> \<sigma>) (embed_eqs U))"
+  proof (induction U)
+    case Nil
+    then show ?case by simp
+  next
+    case (Cons a U)
+    have "m_sapply_eqs \<sigma> (a # U) = (m_sapply_eq \<sigma> a) # (m_sapply_eqs \<sigma> U)" by simp
+    moreover have "m_sapply_eq \<sigma> a = m_eq_of_eq (sapply_eq (embed \<circ> \<sigma>) (embed_eq a))"
+      using link_sapply_eq by blast
+    moreover have "m_sapply_eqs \<sigma> U = m_eqs_of_eqs (sapply_eq_system (embed \<circ> \<sigma>) (embed_eqs U))"
+      using Cons.IH by blast
+    then show ?case
+      by (metis Cons.IH embed_eqs.simps(2) link_sapply_eq m_eqs_of_eqs.simps(2) m_sapply_eqs.simps(2) sapply_eq_system_equiv_def)
+  qed
+
+inductive m_unifies :: "m_subst \<Rightarrow> m_eq \<Rightarrow> bool" where
+  m_unifies_eq: "(m_sapply \<sigma> u = m_sapply \<sigma> t) \<Longrightarrow> m_unifies \<sigma> (u, t)"
+
+lemma link_unifies:
+  "m_unifies \<sigma> eq = unifies (embed \<circ> \<sigma>) (embed_eq eq)"
+  apply (auto simp add: embed_eq.elims fstI link_sapply m_unifies.simps sndI unifies.simps)
+   apply (metis embed_msg_of_term wf_subst_embed wf_term_embed wf_term_sapply)
+  by (metis embed_eq.elims old.prod.inject)
+
+inductive m_unifiess :: "m_subst \<Rightarrow> m_eqs \<Rightarrow> bool" where
+  m_unifiess_empty: "m_unifiess \<sigma> []"
+| m_unifiess_rec:   "(m_unifiess \<sigma> s) \<and> (m_unifies \<sigma> eq) \<Longrightarrow> m_unifiess \<sigma> (eq # s)"
+
+lemma link_unifiess:
+  "m_unifiess \<sigma> U = unifiess (embed \<circ> \<sigma>) (embed_eqs U)"
+  apply (induction U)
+  apply (simp add: m_unifiess_empty unifiess_empty)
+  by (metis (mono_tags, lifting) embed_eqs.simps(2) link_unifies list.discI list.inject m_unifiess.simps unifiess.simps)
+
+fun lift_subst :: "(symbol, string) subst option \<Rightarrow> m_subst option" where
+  "lift_subst None = None"
+| "lift_subst (Some \<sigma>) = Some (msg_of_term \<circ> \<sigma>)"
+
+fun m_unify :: "m_eqs \<Rightarrow> m_subst option" where
+  "m_unify U = lift_subst (unify (embed_eqs U))"
+
+lemma msg_of_term_var[simp]:
+  "msg_of_term \<circ> Unify.Var = msg.Var"
+proof (rule ext)
+  fix x
+  show "(msg_of_term \<circ> term.Var) x = msg.Var x"
+  proof (cases x)
+    case Nil
+    then show ?thesis by simp
+  next
+    case (Cons a list)
+    then show ?thesis by simp
+  qed
+qed
+
+lemma link_unify_1:
+  "m_unify [] = Some Var"
+proof -
+  have "m_unify [] = lift_subst (unify [])" by simp
+  then have "... = lift_subst (Some Unify.Var)" by simp
+  then have "... = Some (msg_of_term \<circ> Unify.Var)" by simp
+  then show ?thesis by simp
+qed
+
+fun m_scomp :: "m_subst \<Rightarrow> m_subst \<Rightarrow> m_subst" (infixl "\<circ>m" 75)
+  where
+  "m_scomp \<sigma> \<tau> = (\<lambda> x. m_sapply \<sigma> (\<tau>(x)))"
+
+fun m_lifted_comp :: "m_subst option \<Rightarrow> m_subst \<Rightarrow> m_subst option"
+  where
+  "m_lifted_comp None \<tau> = None"
+| "m_lifted_comp (Some \<sigma>) \<tau> = Some (\<sigma> \<circ>m \<tau>)"
+
 (*
-    Cons string
-    | Var string
-    | Hash msg
-    | Pair msg msg
-    | Sym_encrypt msg msg
-    | Public_key_encrypt msg msg
-    | Signature msg msg
+lemma link_unify_2:
+  "m_unify ((Var x, t) # U) = (
+  if (x \<notin> m_fv t) then
+    m_lifted_comp (m_unify (m_sapply_eqs (msg.Var(x := t)) U)) (msg.Var(x := t))
+   else (
+     if Var x = t then m_unify U else None
+    )
+  )"
+  sorry
 *)
+
+(*
+function (sequential) m_unify :: "m_eqs \<Rightarrow> m_subst option"
+  where
+  "unify [] = Some Var"
+| "unify ((Var x, t) # U) = (
+| "unify ((u, Var y) # U) = unify ((Var y, u) # U)"
+| "unify ((Fun f u, Fun g v) # U) =
+  (if (f = g \<and> length u = length v) then
+    unify(append (zip u v) U)
+  else
+    None)"
+*)
+
+(*
+fun m_unify :: "m_eqs \<Rightarrow> m_subst option" where
+  "m_unify U = lift_subst (unify (embed_eqs U))"
+*)
+
+(* 5. (e) *)
+
+theorem m_soundness1:
+  assumes "m_unify U = Some \<sigma>"
+  shows "m_unifiess \<sigma> U"
+  using assms
+proof (induction U)
+  case Nil
+  then show ?case
+    by (simp add: m_unifiess_empty)
+next
+  case (Cons a U)
+  obtain \<tau> where "unify (embed_eqs (a # U)) = Some \<tau>"
+    using Cons.prems by fastforce
+  then have "unifiess \<tau> (embed_eqs (a # U))" 
+    by (simp add: soundness1)
+  then have "unifiess \<tau> (embed_eqs U)"
+    by (metis embed_eqs.elims list.discI list.inject local.Cons unifiess.simps)
+  moreover have "\<sigma> = msg_of_term \<circ> \<tau>"
+    using Cons.prems \<open>unify (embed_eqs (a # U)) = Some \<tau>\<close> by auto
+  then show ?case sorry
+qed
+
+(*
+lemma link_unifies:
+  "m_unifies \<sigma> eq = unifies (embed \<circ> \<sigma>) (embed_eq eq)"
+
+lemma link_unifiess:
+  "m_unifiess \<sigma> U = unifiess (embed \<circ> \<sigma>) (embed_eqs U)"
+*)
+
+(*
+  m_unifies_eq: "(m_sapply \<sigma> u = m_sapply \<sigma> t) \<Longrightarrow> m_unifies \<sigma> (u, t)"
+*)
+
+(*
+| m_unifiess_rec:   "(m_unifiess \<sigma> s) \<and> (m_unifies \<sigma> eq) \<Longrightarrow> m_unifiess \<sigma> (eq # s)"
+*)
+
+(* 5. (f) *)
+
+fun m_fv_eq :: "m_eq \<Rightarrow> string set" where
+  "m_fv_eq eq = (m_fv (fst eq)) \<union> (m_fv (snd eq))"
+
+lemma link_fv_eq:
+  "m_fv_eq eq = fv_eq (embed_eq eq)"
+proof -
+  have "m_fv_eq eq = (m_fv (fst eq)) \<union> (m_fv (snd eq))" by simp
+  then have "... = (fv (fst (embed_eq eq))) \<union> (fv (snd (embed_eq eq)))"
+    by (metis embed_eq.simps fstI link_fv prod.collapse sndI)
+  then show ?thesis by simp
+qed
+
+fun m_fv_eqs :: "m_eqs \<Rightarrow> string set" where
+  "m_fv_eqs [] = {}"
+| "m_fv_eqs (eq # U) = (m_fv_eq eq) \<union> (m_fv_eqs U)"
+
+lemma def_equiv:
+  "m_fv_eqs U = (\<Union>x\<in>(set U). m_fv_eq x)"
+proof (induction U)
+  case Nil
+  then show ?case by auto
+next
+  case (Cons a U)
+  then show ?case by simp
+qed
+
+lemma link_fv_eqs:
+  "m_fv_eqs U = fv_eq_system (embed_eqs U)"
+proof (induction U)
+  case Nil
+  have "m_fv_eqs [] = (\<Union>x\<in>(set []). m_fv_eq x)" by simp
+  then have "... = {}" by auto
+  moreover have "embed_eqs [] = []" by simp
+  moreover have "fv_eq_system [] = fold (\<union>) (map fv_eq []) {}" by simp
+  then have "fold (\<union>) (map fv_eq []) {} = fold (\<union>) [] {}" by simp
+  then have "fold (\<union>) [] {} = {}" by simp
+  then show ?case
+    by simp
+next
+  case (Cons a U)
+  then show ?case
+    by (metis embed_eqs.simps(2) fv_eq_system_def_equiv link_fv_eq list.discI list.inject m_fv_eqs.elims)
+qed
+
+fun m_sdom :: "m_subst \<Rightarrow> string set"
+  where
+  "m_sdom \<sigma> = {x. \<sigma> x \<noteq> Var x}"
+
+lemma link_sdom:
+  "m_sdom \<sigma> = sdom (embed \<circ> \<sigma>)"
+proof -
+  have "m_sdom \<sigma> = {x. \<sigma> x \<noteq> msg.Var x}" by auto
+  then have "... = {x. (embed \<circ> \<sigma>) x \<noteq> (embed \<circ> msg.Var) x}"
+    by (metis Collect_cong comp_apply msg_of_term_embed)
+  then show ?thesis by auto
+qed
+
+fun m_sran :: "m_subst \<Rightarrow> msg set"
+  where
+"m_sran \<sigma> = (\<Union>x\<in>m_sdom \<sigma>. {\<sigma> x})"
+
+fun msg_set_of_term_set :: "(symbol, string) term set \<Rightarrow> msg set" where
+  "msg_set_of_term_set s = {msg_of_term x | x. x \<in> s}"
+
+lemma link_sran:
+  "m_sran \<sigma> = msg_set_of_term_set (sran (embed \<circ> \<sigma>))"
+proof -
+  have "m_sran \<sigma> = (\<Union>x\<in>m_sdom \<sigma>. {\<sigma> x})" by simp
+  then have "... = (\<Union>x\<in>(sdom (embed \<circ> \<sigma>)). {\<sigma> x})"
+    using link_sdom by auto
+  then show ?thesis sorry
+qed
+
+fun m_svran:: "m_subst \<Rightarrow> string set"
+  where
+"m_svran \<sigma> = (\<Union>t\<in>(m_sran \<sigma>).(m_fv t))"
+
+lemma link_svran:
+  "m_svran \<sigma> = svran (embed \<circ> \<sigma>)"
+  sorry
+
+lemma m_lemma_3:
+  assumes "m_unify U = Some \<sigma>"
+  shows "m_fv_eqs (m_sapply_eqs \<sigma> U) \<subseteq> m_fv_eqs U"
+    and "m_sdom \<sigma> \<subseteq> m_fv_eqs U"
+    and "m_svran \<sigma> \<subseteq> m_fv_eqs U"
+    and "m_sdom \<sigma> \<inter> m_svran \<sigma> = {}"
+  sorry
 
 end
